Arm/Cosim.lean
@@ -14,7 +14,7 @@ def init_cosim_state : ArmState :=
   { gpr := (fun (_ : BitVec 5) => 0#64),
     sfp := (fun (_ : BitVec 5) => 0#128),
     pc  := 0#64,
-    pstate := (fun (_ : PFlag) => 0#1),
+    pstate := zero_pstate,
     mem := (fun (_ : BitVec 64) => 0#8),
     program := (fun (_ : BitVec 64) => none),
     error := StateError.None }
