Proofs/Sha512_block_armv8.lean
@@ -19,7 +19,7 @@ open BitVec
 
 def sha512_program_test_1 : program :=
   def_program
-   [(0x126538#64 , 0xcec08230#32),      --  sha512su0       v16.2d, v17.2d
+    [(0x126538#64 , 0xcec08230#32),      --  sha512su0       v16.2d, v17.2d
      (0x12653c#64 , 0x6e154287#32),      --  ext     v7.16b, v20.16b, v21.16b, #8
      (0x126540#64 , 0xce6680a3#32),      --  sha512h q3, q5, v6.2d
      (0x126544#64 , 0xce678af0#32)       --  sha512su1       v16.2d, v23.2d, v7.2d
@@ -46,12 +46,11 @@ theorem sha512_program_test_1_sym (s0 s_final : ArmState)
 
 ----------------------------------------------------------------------
 
--- Test 2: We have a 5 instruction program, and we attempt to simulate
--- only 4 of them.
+-- Test 2: A 6 instruction program.
 
 def sha512_program_test_2 : program :=
   def_program
-   [(0x126538#64 , 0xcec08230#32),      --  sha512su0       v16.2d, v17.2d
+    [(0x126538#64 , 0xcec08230#32),      --  sha512su0       v16.2d, v17.2d
      (0x12653c#64 , 0x6e154287#32),      --  ext     v7.16b, v20.16b, v21.16b, #8
      (0x126540#64 , 0xce6680a3#32),      --  sha512h q3, q5, v6.2d
      (0x126544#64 , 0xce678af0#32),      --  sha512su1       v16.2d, v23.2d, v7.2d
@@ -64,15 +63,15 @@ theorem sha512_program_test_2_sym (s0 s_final : ArmState)
   (h_s0_pc : read_pc s0 = 0x126538#64)
   (h_s0_program : s0.program = sha512_program_test_2.find?)
   (h_s0_ok : read_err s0 = StateError.None)
-  (h_run : s_final = run 4 s0) :
+  (h_run : s_final = run 6 s0) :
   read_err s_final = StateError.None := by
   -- Prelude
   simp_all only [state_simp_rules, -h_run]
   -- Symbolic simulation
-  sym_n 4 h_s0_program
+  sym_n 6 h_s0_program
   -- Final steps
   unfold run at h_run
-  subst s_final s_4
+  subst s_final s_6
   simp_all only [state_simp_rules, minimal_theory, bitvec_rules]
   done
 
@@ -82,13 +81,16 @@ theorem sha512_program_test_2_sym (s0 s_final : ArmState)
 
 def sha512_program_test_3 : program :=
   def_program
-  [(0x1264c0#64 , 0xa9bf7bfd#32),      --  stp     x29, x30, [sp, #-16]!
+   [(0x1264c0#64 , 0xa9bf7bfd#32),      --  stp     x29, x30, [sp, #-16]!
     (0x1264c4#64 , 0x910003fd#32),      --  mov     x29, sp
     (0x1264c8#64 , 0x4cdf2030#32),      --  ld1     {v16.16b-v19.16b}, [x1], #64
     (0x1264cc#64 , 0x4cdf2034#32)       --  ld1     {v20.16b-v23.16b}, [x1], #64
   ]
 
-
+-- set_option profiler true in
+-- set_option maxRecDepth 10000 in
+set_option pp.deepTerms false in
+set_option pp.deepTerms.threshold 10 in
 theorem sha512_block_armv8_test_3_sym (s0 s_final : ArmState)
   (h_s0_ok : read_err s0 = StateError.None)
   (h_s0_sp_aligned : CheckSPAlignment s0 = true)
@@ -99,7 +101,36 @@ theorem sha512_block_armv8_test_3_sym (s0 s_final : ArmState)
   -- Prelude
   simp_all only [state_simp_rules, -h_run]
   -- Symbolic simulation
-  -- sym_n 1 h_s0_program
+
+  sym_i_n 0 1 h_s0_program
+
+  -- sym_i_n 1 1 h_s0_program
+  init_next_step h_run
+  rename_i s_2 h_step_2 h_run
+  fetch_and_decode_inst h_step_2 h_s0_program
+  clear h_step_1
+  -- exec_inst h_step_2
+  -- FIXME: simproc for first args. of write_mem_bytes and zeroExtend
+  simp only [exec_inst, DPI.exec_add_sub_imm, write_gpr, Nat.sub_zero, read_gpr, ne_eq,
+    not_false_eq_true, r_of_w_different, r_of_w_same, beq_self_eq_true, ite_true, write_pstate,
+    write_pc, read_pc, w_of_w_shadow, w_program, write_mem_bytes_program, h_s0_program] at h_step_2
+  simp only [beq_iff_eq, ofNat_add_ofNat, Nat.reduceAdd] at h_step_2
+  -- simp (config := {ground := true}) only at h_step_2 -- max. recursion depth is reached.
+  conv at h_step_2 =>
+    rhs
+    arg 3
+    tactic => simp (config := {ground := true}) only [minimal_theory, bitvec_rules, ↓reduceIte, reduceAdd, reduceSub, Fin.reduceEq, Fin.mk_one]
+  (try simp only [BitVec.ofFin_eq_ofNat] at h_step_2)
+
+  -- sym_i_n 2 1 h_s0_program
+  init_next_step h_run
+  rename_i s_3 h_step_3 h_run
+  fetch_and_decode_inst h_step_3 h_s0_program
+  clear h_step_2
+  -- exec_inst h_step_3
+  -- LDST.exec_advanced_simd_multiple_struct_post_indexed
+  simp only [exec_inst, state_simp_rules, minimal_theory, bitvec_rules, ↓reduceIte] at h_step_3
+  -- rw [CheckSPAligment_of_w_different] at h_step_3
   sorry
 
 ----------------------------------------------------------------------
