Tests/SHA512ProgramTest.lean
@@ -585,7 +585,7 @@ def init_sha512_test : ArmState :=
   let s := { gpr := init_gpr,
              sfp := (fun (_ : BitVec 5) => 0#128),
              pc  := 0x1264c0#64,
-             pstate := (fun (_ : PFlag) => 0#1),
+             pstate := zero_pstate,
              mem := (fun (_ : BitVec 64) => 0#8),
              program := sha512_program_map.find?,
              error := StateError.None }
